\section{Theorie}
\label{sec:Theorie}

\begin{equation}
    \label{eq:Fouriersynthese}
    f (t) = \sum_{k=0}^\infty \left(A_k \cos \left( \omega _k t \right) + B_k \sin \left( \omega _k t \right) \right)
\end{equation}

mit

\begin{equation}
    \label{eq:Omega}
    \omega _k = \frac {2 \pi k}{T}
\end{equation}

und

\begin{equation}
    \label{eq:A_k}
    A_k = \frac{2}{T} \int_{\frac{-T}{2}}^{\frac{T}{2}} f(t) \, \cos \left( \omega _k t \right)  \symup{d}t
\end{equation}

mit

\begin{equation}
    \label{eq:A_0}
    A_0 = \frac{1}{T} \int f (t) \, \symup{d}t
\end{equation}

und

\begin{equation}
    \label{eq:B_k}
    B_k = \frac{2}{T} \int_{\frac{-T}{2}}^{\frac{T}{2}} f(t) \, \sin \left( \omega _k t \right)  \symup{d}t
\end{equation}

mit

\begin{equation}
    \label{eq:B_0}
    B_0 = 0
\end{equation}

\cite{sample}
